iodiv/IIOSigSpec.fst
@@ -1,0 +1,40 @@
+module IIOSigSpec
+
+open FStar.List.Tot
+open FStar.List.Tot.Properties
+open FStar.Tactics // Also defines forall_intro so place before Classical
+open FStar.Classical
+open FStar.IndefiniteDescription
+open FStar.Calc
+open FStar.FunctionalExtensionality
+
+open Util
+open Stream
+open IIOSig
+open DivFree
+open DivFreeTauSpec
+open DivFreeTauDM
+
+unfold
+let i_open (s : string) : iwp (either file_descr exn) =
+  as_iwp (fun post hist -> forall fd. post (Ocv [ Some (EOpenfile s fd) ] fd))
+
+unfold
+let i_read (fd : file_descr) : iwp (either string exn) =
+  as_iwp (fun post hist -> is_open fd hist /\ (forall s. post (Ocv [ Some (ERead fd s) ] s)))
+
+unfold
+let i_close (fd : file_descr) : iwp (either unit exn) =
+  as_iwp (fun post hist -> is_open fd hist /\ (forall r. post (Ocv [ Some (EClose fd r) ] r)))
+
+unfold
+let i_get_trace : iwp history =
+  as_iwp (fun post hist -> post (Ocv [] hist))
+
+unfold
+let iodiv_act : action_iwp io_sig =
+  fun ac arg ->
+    match ac with
+    | Openfile -> i_open arg
+    | Read -> i_read arg
+    | Close -> i_close arg
