iodiv/case-study/IIOSig.fst
@@ -1,0 +1,109 @@
+(** (Instrumented) I/O signature *)
+
+module IIOSig
+
+open DivFree
+include Types
+
+type lfds = list file_descr
+
+type iio_act =
+ (* files *)
+ | Openfile 
+ (* file descriptors *)
+ | Read 
+ | Write
+ | Close
+ (* sockets *)
+ | Socket
+ | Setsockopt
+ | Bind
+ | SetNonblock
+ | Listen
+ | Accept
+ | Select
+ (* instrumentation *)
+ | GetTrace
+
+assume val file_descr : eqtype
+
+let not_GetTrace x =
+  match x with
+  | GetTrace -> false
+  | _ -> true
+
+type io_act = ac : iio_act { not_GetTrace ac }
+
+noeq
+type event =
+| EOpenfile : string * (list open_flag) * zfile_perm -> either (file_descr) exn -> event
+| ERead : file_descr * UInt8.t -> either (Bytes.bytes * UInt8.t) exn -> event
+| EWrite : file_descr * Bytes.bytes -> either (unit) exn -> event
+| EClose : file_descr -> either (unit) exn -> event
+| ESocket : unit -> either (file_descr) exn -> event
+| ESetsockopt : file_descr * socket_bool_option * bool -> either (unit) exn -> event
+| EBind : file_descr * string * UInt8.t -> either (unit) exn -> event
+| ESetNonblock : file_descr -> either (unit) exn -> event
+| EListen : file_descr * UInt8.t -> either (unit) exn -> event
+| EAccept : file_descr -> either (file_descr) exn -> event
+| ESelect : lfds * lfds * lfds * UInt8.t -> either (lfds * lfds * lfds ) exn -> event
+
+let trace = list event
+let history = list event // head: latest event
+
+unfold
+let iio_arg ac =
+  match ac with
+  | Openfile -> string * (list open_flag) * zfile_perm
+  | Read -> file_descr * UInt8.t
+  | Write -> file_descr * Bytes.bytes
+  | Close -> file_descr
+  | Socket -> unit
+  | Setsockopt -> file_descr * socket_bool_option * bool
+  | Bind -> file_descr * string * UInt8.t
+  | SetNonblock -> file_descr
+  | Listen -> file_descr * UInt8.t
+  | Accept -> file_descr
+  | Select -> lfds * lfds * lfds * UInt8.t
+  | GetTrace -> unit
+
+unfold
+let iio_res #ac (x : iio_arg ac) =
+  match ac with
+  | Openfile -> either (file_descr) exn
+  | Read -> either (Bytes.bytes * UInt8.t) exn
+  | Write -> either (unit) exn
+  | Close -> either (unit) exn
+  | Socket -> either (file_descr) exn
+  | Setsockopt -> either (unit) exn
+  | Bind -> either (unit) exn
+  | SetNonblock -> either (unit) exn
+  | Listen -> either (unit) exn
+  | Accept -> either (file_descr) exn
+  | Select -> either (lfds * lfds * lfds ) exn
+  | GetTrace -> history
+
+let io_sig : signature = {
+  act = io_act ;
+  arg = iio_arg ;
+  res = iio_res
+}
+
+let iio_sig : signature = {
+  act = iio_act ;
+  arg = iio_arg ;
+  res = iio_res
+}
+
+let rec is_open (fd : file_descr) (hist : history) : bool =
+  match hist with
+  | [] -> false
+  | EClose fd' _ :: hist' ->
+    if fd = fd'
+    then false
+    else is_open fd hist'
+  | EOpenfile s fd' :: hist' ->
+    if Inl? fd' && fd = Inl?.v fd'
+    then true
+    else is_open fd hist'
+  | e :: hist' -> is_open fd hist'
